udpated it_sems_alt1.v, added it_sems_alt1_proof.v (tmp)

proofs/itrees/it_sems_alt1.v
@@ -1,117 +1,35 @@
-
-From Jasmin Require Import oseq.
-(* problematic *)
-From Jasmin Require Import expr.
-From Jasmin Require Import it_jasmin_lib.
-
-(* FIXME clean this *)
-From Coq Require Import
-     Arith.PeanoNat
-     Lists.List
-     Strings.String
-     Morphisms
-     Setoid
-     RelationClasses
-     EquivDec
-     Equality
-     Program.Tactics.
-
-From ExtLib Require Import
-     Data.String
-     Structures.Monad
-     Structures.Traversable
-     Data.List
-     Core.RelDec
-     Structures.Maps
-     Data.Map.FMapAList.
-
 From ITree Require Import
      ITree
      ITreeFacts
-     Monad
-     Basics.HeterogeneousRelations
-     Events.Map
-     Events.State
-     Events.StateFacts
-     Events.Reader
      Events.Exception
-     Events.FailFacts.
-
-Require Import Paco.paco.
-Require Import Psatz.
-Require Import ProofIrrelevance.
-Require Import FunctionalExtensionality.
-
-From mathcomp Require Import ssreflect ssrfun ssrbool ssrnat seq eqtype fintype.
-
-From ITree Require Import
-     Basics.Category
-     Basics.Basics
-     Basics.Function
-     Core.ITreeDefinition
-     Core.KTree
-     Eq.Eqit
-     Eq.UpToTaus
-     Eq.Paco2
-     Indexed.Sum
-     Indexed.Function
-     Indexed.Relation
-     Interp.Handler
-     Interp.Interp
-     Interp.InterpFacts
      Interp.Recursion.
 
-From ITree Require Import Rutt RuttFacts.
+From mathcomp Require Import ssreflect ssrfun ssrbool eqtype.
 
-From ITree Require Import EqAxiom.
+Require Import expr psem_defs psem it_gen_lib it_exec.
 
-From Jasmin Require Import expr psem_defs psem oseq.
-From Jasmin Require Import it_gen_lib it_jasmin_lib it_exec.
-From Jasmin Require Import compiler_util.
-(* problematic *)
-
-(* End FIXME *)
-Import Monads.
 Import MonadNotation.
 Local Open Scope monad_scope.
-Local Open Scope option_scope.
 
 Set Implicit Arguments.
 Unset Strict Implicit.
 Unset Printing Implicit Defensive.
 
-(* Set Universe Polymorphism. *)
-
-(* This files contains semantic models distinguished by use of either
-mutual or double recursion, and by either modular, error-aware or flat
-structure. There are fives models (MM: mutual modular; ME: mutual
-error; MF: mutual flat; DE: double error; DF double flat) *)
-
 (**** ERROR SEMANTICS *******************************************)
 Section Errors.
 
-(* type of errors (this might becom richer) *)
-  (* Variant ErrType : Type := Err : ErrType. *)
 (* error events *)
-
-
 Definition ErrEvent : Type -> Type := exceptE error_data.
 
-(*
-sem_I : prog -> estate -> instr -> itree syscall_Event (state_error + estate)
-sem_i : prog -> estate -> instr_r -> itree syscall_Event (state_error + estate)
-sem_c : prog -> estate -> cmd -> itree syscall_Event (state_error + estate)
-sem_fun : prog -> mem -> syscall -> funname -> values -> itree syscall_Event (state_error + (mem * syscall * values))
-*)
-
-(* failT (itree E) R = itree E (option R) *)
+(* maps ErrEvent events to the execS datatype *)
+(* execT (itree E) R = itree E (execS R) *)
 Definition handle_Err {E} : ErrEvent ~> execT (itree E) :=
   fun _ e =>
     match e with
     | Throw e' => Ret (ESerror _ e')
     end.
 
-(* Err handler *)
+(* ErrEvent handler *)
 Definition ext_handle_Err {E: Type -> Type} :
   ErrEvent +' E ~> execT (itree E) :=
   fun _ e =>
@@ -126,14 +44,15 @@ Definition interp_Err {E: Type -> Type} {A}
 
 (*** auxiliary error functions *)
 
-Definition ioget {E: Type -> Type} `{ErrEvent -< E} {V} (err: error_data) (o: option V) : itree E V :=
+Definition ioget {E: Type -> Type} `{ErrEvent -< E} {V}
+  (err: error_data) (o: option V) : itree E V :=
   match o with
   | Some v => Ret v
   | None => throw err
   end.
 
-Definition err_result {E: Type -> Type} `{ErrEvent -< E} (Err : error -> error_data) :
-  result error ~> itree E :=
+Definition err_result {E: Type -> Type} `{ErrEvent -< E}
+  (Err : error -> error_data) : result error ~> itree E :=
   fun _ t => match t with
              | Ok v => Ret v
              | Error e => throw (Err e) end.
@@ -143,7 +62,6 @@ End Errors.
 Section WSW.
 Context
   {asm_op: Type}
-  {asmop: asmOp asm_op}
   {wsw: WithSubWord}
   {dc: DirectCall}
   {syscall_state : Type}
@@ -151,133 +69,152 @@ Context
   {spp : SemPexprParams}
   {sip : SemInstrParams asm_op syscall_state}
   {pT : progT}
-  {scP : semCallParams}
-  (pr : prog)
-  (ev : extra_val_t).
+  {scP : semCallParams}.
 
 Definition mk_error_data (s:estate) (e:error)  := (e, tt).
 
 Definition mk_errtype := fun s => mk_error_data s ErrType.
 
-Definition iget_fundef {E} `{ErrEvent -< E}
-  (fn: funname) (s:estate) : itree E fundef :=
-  ioget (mk_errtype s) (get_fundef (p_funcs pr) fn).
+Section CORE.
 
-Definition iresult  {E} `{ErrEvent -< E} {T} (s:estate) (F : exec T)  : itree E T :=
+Context {E} `{ErrEvent -< E} (p : prog) (ev : extra_val_t).
+
+Definition iget_fundef (funcs: fun_decls) (fn: funname) (s:estate) : itree E fundef :=
+  ioget (mk_errtype s) (get_fundef funcs fn).
+
+Definition iresult {T} (s:estate) (F : exec T)  : itree E T :=
   err_result (mk_error_data s) F.
 
-Definition iwrite_var {E} `{ErrEvent -< E}
-   (wdb : bool) (x : var_i) (v : value) (s : estate) : itree E estate :=
+Definition iwrite_var (wdb : bool) (x : var_i) (v : value) (s : estate) : itree E estate :=
   iresult s (write_var wdb x v s).
 
-Definition iwrite_lval {E} `{ErrEvent -< E}
-   (wdb : bool) (gd : glob_decls) (x : lval) (v : value) (s : estate) : itree E estate :=
+Definition iwrite_lval (wdb : bool) (gd : glob_decls) (x : lval) (v : value) (s : estate) : itree E estate :=
   iresult s (write_lval wdb gd x v s).
 
-Definition iwrite_lvals {E} `{ErrEvent -< E}
-   (wdb : bool) (gd : glob_decls) (s : estate) (xs : lvals) (vs : values) : itree E estate :=
+Definition iwrite_lvals (wdb : bool) (gd : glob_decls) (s : estate) (xs : lvals) (vs : values) : itree E estate :=
   iresult s (write_lvals wdb gd s xs vs).
 
-Definition isem_pexpr {E} `{ErrEvent -< E}
-   (wdb : bool) (gd : glob_decls) (s : estate) (e: pexpr) : itree E value :=
+Definition isem_pexpr (wdb : bool) (gd : glob_decls) (s : estate) (e: pexpr) : itree E value :=
   iresult s (sem_pexpr wdb gd s e).
 
-Definition isem_pexprs {E} `{ErrEvent -< E}
-   (wdb : bool) (gd : glob_decls) (s : estate) (es: pexprs) : itree E values :=
+Definition isem_pexprs (wdb : bool) (gd : glob_decls) (s : estate) (es: pexprs) : itree E values :=
   iresult s (sem_pexprs wdb gd s es).
 
-Definition eval_assgn
-  (x: lval) (tg: assgn_tag) (ty: stype) (e: pexpr)
-  (st1: estate) : exec estate :=
-   (Let v := sem_pexpr true (p_globs pr) st1 e in
+Definition sem_assgn  (x : lval) (tg : assgn_tag) (ty : stype) (e : pexpr) (s : estate) : exec estate :=
+   (Let v := sem_pexpr true (p_globs p) s e in
     Let v' := truncate_val ty v in
-    write_lval true (p_globs pr) x v' st1).
+    write_lval true (p_globs p) x v' s).
 
-Definition eval_syscall
-   (xs: lvals) (o: syscall_t)
-   (es: pexprs) (s: estate) : exec estate :=
-  Let ves := sem_pexprs true (p_globs pr) s es in
-  Let: (scs, m, vs) := exec_syscall s.(escs) s.(emem) o ves in
-  write_lvals true (p_globs pr)
-     (with_scs (with_mem s m) scs) xs vs.
+Record fstate := { fscs : syscall_state_t; fmem : mem; fvals : values }.
 
-(** Auxiliary functions for recursion on list (seq) *)
+Definition fexec_syscall (o : syscall_t) (fs:fstate) : exec fstate :=
+  Let: (scs, m, vs) := exec_syscall fs.(fscs) fs.(fmem) o fs.(fvals) in
+  ok {| fscs := scs; fmem := m; fvals := vs |}.
 
-Fixpoint isem_map {E} (sem_i: instr -> estate -> itree E estate)
-   (c: cmd) (st: estate) : itree E estate :=
+Definition mk_fstate (vs:values) (s:estate) := {| fscs := escs s; fmem:= emem s; fvals := vs |}.
+
+Definition upd_estate wdb (gd : glob_decls) (xs:lvals) (fs : fstate) (s:estate) :=
+  write_lvals wdb gd (with_scs (with_mem s fs.(fmem)) fs.(fscs)) xs fs.(fvals).
+
+Definition sem_syscall (xs : lvals) (o : syscall_t) (es : pexprs) (s : estate) : exec estate :=
+  Let ves := sem_pexprs true (p_globs p) s es in
+  Let fs := fexec_syscall o (mk_fstate ves s) in
+  upd_estate true (p_globs p) xs fs s.
+
+Definition sem_cond (gd : glob_decls) (e : pexpr) (s : estate) : exec bool :=
+  sem_pexpr true gd s e >>r= to_bool.
+
+Definition isem_cond (e : pexpr) (s : estate) : itree E bool :=
+  iresult s (sem_cond (p_globs p) e s).
+
+Definition sem_bound (gd : glob_decls) (lo hi : pexpr) (s : estate) : exec (Z * Z) :=
+  Let vlo := sem_pexpr true gd s lo >>r= to_int in
+  Let vhi := sem_pexpr true gd s hi >>r= to_int in
+  ok (vlo, vhi).
+
+Definition isem_bound (lo hi : pexpr) (s : estate) : itree E (Z * Z) :=
+  iresult s (sem_bound (p_globs p) lo hi s).
+
+End CORE.
+
+Section SEM_C.
+
+Context {E} `{ErrEvent -< E}
+        (sem_i: prog -> extra_val_t -> instr -> estate -> itree E estate)
+        (p : prog) (ev : extra_val_t).
+
+(* isem_cmd_body *)
+Fixpoint isem_map (c: cmd) (s: estate) : itree E estate :=
   match c with
-  | nil => Ret st
-  | i :: c' => st' <- sem_i i st ;; isem_map sem_i c' st'
+  | nil => Ret s
+  | i :: c' => s' <- sem_i p ev i s ;; isem_map c' s'
   end.
 
-Fixpoint isem_for_body {E} `{ErrEvent -< E}
-   (sem_i : instr -> estate -> itree E estate)
-   (i: var_i) (c: cmd)
-   (ls: list Z) (s: estate) : itree E estate :=
+Fixpoint isem_for_body (i : var_i) (c : cmd) (ls : list Z) (s : estate) : itree E estate :=
   match ls with
   | nil => ret s
   | (w :: ws) =>
     s <- iwrite_var true i (Vint w) s;;
-    s <- isem_map sem_i c s;;
-    isem_for_body sem_i i c ws s
+    s <- isem_map c s;;
+    isem_for_body i c ws s
   end.
 
 (* Make global definition *)
 Local Notation continue_loop st := (ret (inl st)).
 Local Notation exit_loop st := (ret (inr st)).
 
-Local Notation gd := (p_globs pr).
-
-Definition isem_cond {E} `{ErrEvent -< E} (e:pexpr) (s: estate) : itree E bool :=
-  iresult s (sem_pexpr true gd s e >>r= to_bool).
-
-Definition isem_bound {E} `{ErrEvent -< E} (e:pexpr) (s: estate) :
-   itree E Z :=
-  iresult s (sem_pexpr true gd s e >>r= to_int).
-
-Definition isem_while_body {E} `{ErrEvent -< E}
-   (sem_i : instr -> estate -> itree E estate)
-   (c1 : cmd) (e:pexpr) (c2: cmd) (s1 : estate) : itree E (estate + estate) :=
-   s2 <- isem_map sem_i c1 s1 ;;
-   b <- isem_cond e s2 ;;
-   if b then s3 <- isem_map sem_i c2 s2 ;; continue_loop s3
+Definition isem_while_loop (c1 : cmd) (e : pexpr) (c2 : cmd) (s1 : estate) : itree E (estate + estate) :=
+   s2 <- isem_map c1 s1 ;;
+   b <- isem_cond p e s2 ;;
+   if b then s3 <- isem_map c2 s2 ;; continue_loop s3
    else exit_loop s2.
 
-Definition isem_while {E} `{ErrEvent -< E}
-   (sem_i : instr -> estate -> itree E estate)
-   (c1 : cmd) (e:pexpr) (c2: cmd) (s1 : estate) : itree E estate :=
-  ITree.iter (isem_while_body sem_i c1 e c2) s1.
+Definition isem_while (c1 : cmd) (e:pexpr) (c2: cmd) (s1 : estate) : itree E estate :=
+  ITree.iter (isem_while_loop c1 e c2) s1.
 
-Record fstate := { fscs : syscall_state_t; fmem : mem; fvals : values }.
+End SEM_C.
 
-Fixpoint isem_i_body {E} `{ErrEvent -< E}
-   (sem_call : funname -> fstate -> itree E fstate)
-   (i: instr) (s1: estate) : itree E estate :=
-  let sem_i := isem_i_body sem_call in
-  let sem_cmd := isem_map sem_i in
+Section SEM_I.
+
+Context {E} `{ErrEvent -< E} 
+  (sem_fun : prog -> extra_val_t -> funname -> fstate -> itree E fstate).
+
+Fixpoint isem_i_body (p : prog) (ev : extra_val_t)
+  (i : instr) (s1 : estate) : itree E estate :=
   let: (MkI _ i) := i in
   match i with
-  | Cassgn x tg ty e => iresult s1 (eval_assgn x tg ty e s1)
-  | Copn xs tg o es => iresult s1 (sem_sopn gd o s1 xs es)
-  | Csyscall xs o es => iresult s1 (eval_syscall xs o es s1)
+  | Cassgn x tg ty e => iresult s1 (sem_assgn p x tg ty e s1)
+  | Copn xs tg o es => iresult s1 (sem_sopn (p_globs p) o s1 xs es)
+  | Csyscall xs o es => iresult s1 (sem_syscall p xs o es s1)
 
   | Cif e c1 c2 =>
-    b <- isem_cond e s1;;
-    sem_cmd (if b then c1 else c2) s1
+    b <- isem_cond p e s1;;
+    isem_map isem_i_body p ev (if b then c1 else c2) s1
 
   | Cwhile a c1 e c2 =>
-    isem_while sem_i c1 e c2 s1
+    isem_while isem_i_body p ev c1 e c2 s1
 
   | Cfor i (d, lo, hi) c =>
-    vlo <- isem_bound lo s1 ;;
-    vhi <- isem_bound hi s1 ;;
-    isem_for_body sem_i i c (wrange d vlo vhi) s1
+    bounds <- isem_bound p lo hi s1 ;;
+    isem_for_body isem_i_body p ev i c (wrange d bounds.1 bounds.2) s1
 
   | Ccall xs fn args =>
-    vargs <- isem_pexprs  (~~direct_call) gd s1 args;;
-    r <- sem_call fn {| fscs := escs s1; fmem:= emem s1; fvals := vargs |} ;;
-    iwrite_lvals (~~direct_call) gd (with_scs (with_mem s1 r.(fmem)) r.(fscs)) xs r.(fvals)
+    vargs <- isem_pexprs  (~~direct_call) (p_globs p) s1 args;;
+    fs <- sem_fun p ev fn (mk_fstate vargs s1) ;;
+    iresult s1 (upd_estate (~~direct_call) (p_globs p) xs fs s1)
   end.
+
+Definition isem_cmd_ := isem_map isem_i_body.
+
+Lemma isem_cmd_cat p ev c c' s :
+  isem_cmd_ p ev (c ++ c') s ≈ (s' <- isem_cmd_ p ev c s;; isem_cmd_ p ev c' s').
+Proof.
+  rewrite /isem_cmd_; elim: c s => [ | i c hc] /= s.
+  + rewrite bind_ret_l; reflexivity.
+  rewrite bind_bind; setoid_rewrite hc; reflexivity.
+Qed.
+
+End SEM_I.
 
 (**********************************************************************)
 (** error-aware interpreter with mutual recursion *)
@@ -285,111 +222,73 @@ Fixpoint isem_i_body {E} `{ErrEvent -< E}
 Definition estate0 (fs : fstate) :=
   Estate fs.(fscs) fs.(fmem) Vm.init.
 
-Definition initialize_call (fd:fundef) (fs:fstate) : exec estate :=
+Definition initialize_funcall (p : prog) (ev : extra_val_t) (fd : fundef) (fs : fstate) : exec estate :=
   let sinit := estate0 fs in
   Let vargs' := mapM2 ErrType dc_truncate_val fd.(f_tyin) fs.(fvals) in
-  Let s0 := init_state fd.(f_extra) (p_extra pr) ev sinit in
+  Let s0 := init_state fd.(f_extra) (p_extra p) ev sinit in
   write_vars (~~direct_call) fd.(f_params) vargs' s0.
 
-Definition finalize_call (fd : fundef) (s:estate) :=
+Definition finalize_funcall (fd : fundef) (s:estate) :=
   Let vres := get_var_is (~~ direct_call) s.(evm) fd.(f_res) in
   Let vres' := mapM2 ErrType dc_truncate_val fd.(f_tyout) vres in
   let scs := s.(escs) in
   let m := finalize fd.(f_extra) s.(emem) in
   ok {| fscs := scs; fmem := m; fvals := vres' |}.
 
-Definition isem_call_body {E} `{ErrEvent -< E}
-   (rec_call : funname -> fstate -> itree E fstate)
-   (fn : funname) (fs:fstate) : itree E fstate :=
+Definition isem_funcall {E} `{ErrEvent -< E}
+   (rec_call : prog -> extra_val_t -> funname -> fstate -> itree E fstate)
+   (p : prog) (ev : extra_val_t)
+   (fn : funname) (fs : fstate) : itree E fstate :=
   (* FIXME: this is durty : sinit*)
   let sinit := estate0 fs in
-  fd <- iget_fundef fn sinit;;
-  s1 <- iresult sinit (initialize_call fd fs);;
-  s2 <- isem_map (isem_i_body rec_call) fd.(f_body) s1;;
-  iresult s2 (finalize_call fd s2).
-
-Notation it_rec_call := (trigger_inl1). 
-
-Notation CALL := (callE (funname * fstate) fstate).
-
-Definition isem_fcallY {E}
-    (fn: funname) (fc: fstate) : itree (CALL +' E) fstate :=
-  trigger (Call (fn, fc)).
-
-Definition isem_call_bodyY {E} `{ErrEvent -< E}                        
-   (fn : funname) (fs:fstate) : itree (CALL +' E) fstate :=
-  (* FIXME: this is durty : sinit*)
-  let sinit := estate0 fs in
-  fd <- iget_fundef fn sinit;;
-  s1 <- iresult sinit (initialize_call fd fs);;
-  s2 <- isem_map (isem_i_body isem_fcallY) fd.(f_body) s1;;
-  iresult s2 (finalize_call fd s2).
-
-Definition isem_callY {E} `{ErrEvent -< E}
-  (fn : funname) (fs : fstate) :
-  itree E fstate :=
-  rec (fun x => isem_call_bodyY (fst x) (snd x)) (fn, fs).
-
-Definition isem_i {E} `{ErrEvent -< E} (i : instr) (s : estate) :
-  itree E estate :=
-  isem_i_body isem_callY i s.
-
-Definition isem_cmd {E} `{ErrEvent -< E} (c : cmd) (s : estate) :
-  itree E estate :=
-  isem_map isem_i c s.
-
-Definition sem_call (fn : funname) (fs : fstate) :
-  execT (itree void1) (fstate) :=
-  interp_Err (isem_callY fn fs).
+  fd <- iget_fundef (p_funcs p) fn sinit;;
+  s1 <- iresult sinit (initialize_funcall p ev fd fs);;
+  s2 <- isem_cmd_ rec_call p ev fd.(f_body) s1;;
+  iresult s2 (finalize_funcall fd s2).
 
 
-Lemma interp_isem_cmd {E} `{ErrEvent -< E} c s :
-  eutt (E:=E) eq (interp (mrecursive it_rec_call) (isem_map (isem_i_body isem_fcallY) c s))
-    (isem_map (isem_i_body isem_callY) c s).
+Section SEM_F.
 
-  
-(********************************************************************************************)
-  
-(* callE (funname * fstate) fstate : Type -> Type :=
-   | Call : (funname * fstate) -> callE (funname * fstate) fstate fstate.
-*)
-Variant recCall : Type -> Type :=
- | RecCall (f:funname) (fs:fstate) : recCall fstate.
+Context {E} `{ErrEvent -< E}.
 
-(* Make global definition *)
+Notation recCall := (callE (funname * fstate) fstate).
 
-Definition rec_call {E} (f:funname) (fs:fstate) : itree (recCall +' E) fstate :=
- trigger_inl1 (RecCall f fs).
+Definition rec_call (p : prog) (ev : extra_val_t) (fn: funname) (fc: fstate) :
+  itree (recCall +' E) fstate := trigger (Call (fn, fc)).
 
-Definition isem_i_rec {E} `{ErrEvent -< E} (i : instr) (s1: estate) : itree (recCall +' E) estate :=
-  isem_i_body rec_call i s1.
+Definition isem_i_rec (p : prog) (ev : extra_val_t) (i : instr) (s1 : estate) : itree (recCall +' E) estate :=
+  isem_i_body rec_call p ev i s1.
 
-Definition isem_call_rec {E} `{ErrEvent -< E}
-   (fn : funname) (fs:fstate) : itree (recCall +' E) fstate :=
-  isem_call_body rec_call fn fs.
+Definition isem_cmd_rec (p : prog) (ev : extra_val_t) (c : cmd) (s1 : estate) : itree (recCall +' E) estate :=
+  isem_cmd_ rec_call p ev c s1.
 
-Definition interp_recCall {E} `{ErrEvent -< E} : recCall ~> itree (recCall +' E) :=
- fun T (rc : recCall T) =>
-   match rc with
-   | RecCall fn fs => isem_call_rec fn fs
-   end.
+Definition isem_fun_rec (p : prog) (ev : extra_val_t)
+   (fn : funname) (fs : fstate) : itree (recCall +' E) fstate :=
+  isem_funcall rec_call p ev fn fs.
 
-Definition isem_call {E} `{ErrEvent -< E} (fn : funname) (fs : fstate) : itree E fstate :=
-  mrec interp_recCall (RecCall fn fs).
+Definition handle_recCall 
+  (p : prog) (ev : extra_val_t) (x: funname * fstate) :
+  itree (recCall +' E) fstate :=
+  isem_fun_rec p ev (fst x) (snd x).
 
-Definition isem_i {E} `{ErrEvent -< E} (i : instr) (s : estate) : itree E estate :=
-  isem_i_body isem_call i s.
+Definition isem_fun (p : prog) (ev : extra_val_t) (fn : funname) (fs : fstate) : itree E fstate :=
+  rec (handle_recCall p ev) (fn, fs).
 
-Definition isem_cmd {E} `{ErrEvent -< E} (c : cmd) (s : estate) : itree E estate :=
-  isem_map isem_i c s.
+Definition isem_i (p : prog) (ev : extra_val_t) (i : instr) (s : estate) : itree E estate :=
+  isem_i_body isem_fun p ev i s.
 
-Definition sem_call (fn : funname) (fs : fstate) : execT (itree void1) (fstate) :=
-  interp_Err (isem_call fn fs).
+Definition isem_cmd (p : prog) (ev : extra_val_t) (c : cmd) (s : estate) : itree E estate :=
+  isem_cmd_ isem_fun p ev c s.
+
+End SEM_F.
+
+Definition sem_fun (p : prog) (ev : extra_val_t) (fn : funname) (fs : fstate) : execT (itree void1) (fstate) :=
+  interp_Err (isem_fun p ev fn fs).
 
 (* Core lemmas about the definition *)
 
-Lemma interp_ioget {E : Type -> Type} `{ErrEvent -< E} Err T (o : option T) :
-  eutt (E:=E) eq (interp (mrecursive interp_recCall) (ioget Err o)) (ioget Err o).
+Lemma interp_ioget {E : Type -> Type} `{ErrEvent -< E} (p : prog) (ev : extra_val_t) Err T (o : option T) :
+  eutt (E:=E) eq (interp (recursive (handle_recCall p ev)) (ioget Err o)) (ioget Err o).
 Proof.
   case o => /=.
   + move=> ?; rewrite interp_ret; reflexivity.
@@ -397,8 +296,8 @@ Proof.
   by apply eqit_Vis => -[].
 Qed.
 
-Lemma interp_iresult {E : Type -> Type} `{ErrEvent -< E} s T (r : exec T) :
-  eutt (E:=E) eq (interp (mrecursive interp_recCall) (iresult s r)) (iresult s r).
+Lemma interp_iresult {E : Type -> Type} `{ErrEvent -< E} (p : prog) (ev : extra_val_t) s T (r : exec T) :
+  eutt (E:=E) eq (interp (recursive (handle_recCall p ev)) (iresult s r)) (iresult s r).
 Proof.
   case r => /=.
   + move=> ?; rewrite interp_ret; reflexivity.
@@ -406,21 +305,22 @@ Proof.
   by apply eqit_Vis => -[].
 Qed.
 
-Lemma interp_isem_cmd {E} `{ErrEvent -< E} c s :
-  eutt (E:=E) eq (interp (mrecursive interp_recCall) (isem_map (isem_i_body rec_call) c s))
-    (isem_map (isem_i_body isem_call) c s).
+Lemma interp_isem_cmd {E} `{ErrEvent -< E} (p : prog) (ev : extra_val_t) c s :
+  eutt (E:=E) eq (interp (recursive (handle_recCall p ev)) (isem_map isem_i_rec p ev c s))
+         (isem_map (isem_i_body isem_fun) p ev c s).
 Proof.
-  apply: (cmd_rect
+  apply:
+   (cmd_rect
     (Pr := fun ir => forall ii s,
-       eutt (E:=E) eq (interp (mrecursive interp_recCall) (isem_i_rec (MkI ii ir) s))
-                      (isem_i (MkI ii ir) s))
+       eutt (E:=E) eq (interp (recursive (handle_recCall p ev)) (isem_i_rec p ev (MkI ii ir) s))
+                      (isem_i p ev (MkI ii ir) s))
     (Pi := fun i => forall s,
-       eutt (E:=E) eq (interp (mrecursive interp_recCall) (isem_i_rec i s))
-                      (isem_i i s))
+       eutt (E:=E) eq (interp (recursive (handle_recCall p ev)) (isem_i_rec p ev i s))
+                      (isem_i p ev i s))
     (Pc := fun c => forall s,
-       eutt (E:=E) eq (interp (mrecursive interp_recCall) (isem_map isem_i_rec c s))
-                      (isem_cmd c s))) c s => //=.
-  + move=> s; rewrite interp_ret; reflexivity.
+       eutt (E:=E) eq (interp (recursive (handle_recCall p ev)) (isem_map isem_i_rec p ev c s))
+                      (isem_cmd p ev c s))) => // {c s}.
+  + move=> s /=; rewrite interp_ret; reflexivity.
   + move=> i c hi hc s; rewrite interp_bind;apply eqit_bind; first by apply hi.
     by move=> s'; apply hc.
   + by move=> >; apply interp_iresult.
@@ -432,9 +332,7 @@ Proof.
     by move=> []; [apply hc1 | apply hc2].
   + move=> v dir lo hi c hc ii s; rewrite /isem_i /isem_i_rec /=.
     rewrite interp_bind; apply eqit_bind; first by apply interp_iresult.
-    move=> vlo.
-    rewrite interp_bind; apply eqit_bind; first by apply interp_iresult.
-    move=> vhi; elim: wrange s => {vlo vhi ii} //=.
+    move=> bounds; elim: wrange s => {bounds ii} //=.
     + move=> >; rewrite interp_ret; reflexivity.
     move=> j js hrec s.
     rewrite interp_bind; apply eqit_bind; first by apply interp_iresult.
@@ -442,7 +340,7 @@ Proof.
     rewrite hc; setoid_rewrite hrec; reflexivity.
   + move=> al c1 e c2 hc1 hc2 ii s; rewrite /isem_i /isem_i_rec /= /isem_while.
     rewrite interp_iter; apply eutt_iter => {}s.
-    rewrite /isem_while_body.
+    rewrite /isem_while_loop.
     rewrite interp_bind; apply eqit_bind; first by apply hc1.
     move=> s1; rewrite interp_bind; apply eqit_bind; first by apply interp_iresult.
     move=> [].
@@ -453,15 +351,15 @@ Proof.
   rewrite interp_bind; apply eqit_bind; first by apply interp_iresult.
   move=> vs.
   rewrite interp_bind; apply eqit_bind; last by move=> >; apply interp_iresult.
-  rewrite interp_mrecursive; reflexivity.
+  rewrite interp_recursive_call; reflexivity.
 Qed.
 
-Lemma isem_call_unfold {E} `{ErrEvent -< E} (fn : funname) (fs : fstate) :
-  isem_call (E:=E) fn fs ≈ isem_call_body isem_call fn fs.
+Lemma isem_call_unfold {E} `{ErrEvent -< E} (p : prog) (ev : extra_val_t) (fn : funname) (fs : fstate) :
+  isem_fun (E:=E) p ev fn fs ≈ isem_funcall isem_fun p ev fn fs.
 Proof.
-  rewrite {1}/isem_call.
-  rewrite mrec_as_interp.
-  rewrite {2}/interp_recCall /isem_call_rec /isem_call_body.
+  rewrite {1}/isem_fun.
+  rewrite rec_as_interp.
+  rewrite {2}/handle_recCall /isem_fun_rec /isem_funcall.
   rewrite interp_bind; apply eqit_bind.
   + by apply interp_ioget.
   move=> fd; rewrite interp_bind; apply eqit_bind.
@@ -472,5 +370,3 @@ Proof.
 Qed.
 
 End WSW.
-
-
