proofs/itrees/it_sems_alt1_proof.v
@@ -1,0 +1,1059 @@
+From Coq Require Import
+     Arith.PeanoNat
+     Lists.List
+     Strings.String
+     Morphisms
+     Setoid
+     RelationClasses
+     EquivDec
+     Equality
+     Program.Tactics.
+
+From ExtLib Require Import
+     Data.String
+     Structures.Monad
+     Structures.Traversable
+     Data.List
+     Core.RelDec
+     Structures.Maps
+     Data.Map.FMapAList.
+
+From ITree Require Import
+     ITree
+     ITreeFacts
+     Monad
+     Basics.HeterogeneousRelations
+     Events.Map
+     Events.State
+     Events.StateFacts
+     Events.Reader
+     Events.Exception
+     Events.FailFacts.
+
+Require Import Paco.paco.
+Require Import Psatz.
+Require Import ProofIrrelevance.
+Require Import FunctionalExtensionality.
+
+From mathcomp Require Import ssreflect ssrfun ssrbool ssrnat seq eqtype fintype.
+
+From ITree Require Import
+(*     Basics.Tacs *)
+     Basics.Category
+     Basics.Basics
+     Basics.Function
+     Core.ITreeDefinition
+     Core.KTree
+     Eq.Eqit
+     Eq.UpToTaus
+     Eq.Paco2
+     Indexed.Sum
+     Indexed.Function
+     Indexed.Relation
+     Interp.Handler
+     Interp.Interp
+     Interp.InterpFacts
+     Interp.Recursion.
+
+From ITree Require Import XRutt XRuttFacts.
+
+From ITree Require Import EqAxiom.
+
+From Jasmin Require Import expr psem_defs psem oseq compiler_util xrutt_aux.
+From Jasmin Require Import it_gen_lib it_jasmin_lib it_sems_alt1.
+
+Import Monads.
+Import MonadNotation.
+Local Open Scope monad_scope.
+Local Open Scope option_scope.
+
+Set Implicit Arguments.
+Unset Strict Implicit.
+Unset Printing Implicit Defensive.
+
+(* PROBLEM with sections *)
+
+(* This files contains proofs to test the semantic models in
+ it_sems. It turns out that double recursion leads to a duplication of
+ inductive proofs, and thus that mutual recursion leads to simpler
+ proofs. The proofs on the modular model are still based on eutt and
+ need to be revised. The proofs on the flat models are much longer and
+ more laden with detail than those on the error-aware model. *)
+
+Class with_Error (E: Type -> Type) {HasErr: ErrEvent -< E} := {
+  is_error : forall {X}, E X -> bool;
+  is_error_has : forall {X} (e:ErrEvent X) , is_error (HasErr X e)
+}.
+Arguments with_Error : clear implicits.
+Arguments with_Error E {_}.
+
+Definition ErrorCutoff {E: Type -> Type} {HasErr: ErrEvent -< E} {wE : with_Error E} X (m : E X) :=
+  ~~(is_error m).
+
+Definition NoCutoff {E: Type -> Type} {HasErr: ErrEvent -< E} {wE : with_Error E} X (m : E X) := true.
+
+Definition rutt_err {E1 E2: Type -> Type}
+  {HasErr1: ErrEvent -< E1} {wE1 : with_Error E1}
+  {HasErr2: ErrEvent -< E2} {wE2 : with_Error E2}
+  {O1 O2 : Type}
+  (RpreInv : prerel E1 E2)
+  (RpostInv: postrel E1 E2)
+  (post      : O1 -> O2 -> Prop) :=
+  @rutt E1 E2 O1 O2 ErrorCutoff NoCutoff RpreInv RpostInv post.
+
+Instance with_Error_suml {E: Type -> Type} {HasErr: ErrEvent -< E} {wE : with_Error E} (T:Type -> Type) :
+  with_Error (T +' E).
+Proof.
+  apply (@Build_with_Error _ _  (EE_MR (fun X (e: E X) => is_error e) T)).
+  move=> x e => /=.
+  apply is_error_has.
+Defined.
+
+Lemma interp_mrec_rutt_err {D1 D2 E1 E2 : Type -> Type}
+   {HasErr1: ErrEvent -< E1} {wE1 : with_Error E1}
+   {HasErr2: ErrEvent -< E2} {wE2 : with_Error E2}
+   (RPre : prerel E1 E2)
+   (RPreInv : prerel D1 D2)
+   (RPost : postrel E1 E2)
+   (RPostInv : postrel D1 D2)
+   (bodies1 : forall T : Type, D1 T -> itree (D1 +' E1) T)
+   (bodies2 : forall T : Type, D2 T -> itree (D2 +' E2) T):
+   (forall (R1 R2 : Type) (d1 : D1 R1) (d2 : D2 R2),
+       RPreInv R1 R2 d1 d2 -> rutt_err (sum_prerel RPreInv RPre) (sum_postrel RPostInv RPost) (fun v1 : R1 => [eta RPostInv R1 R2 d1 v1 d2]) (bodies1 R1 d1) (bodies2 R2 d2)) ->
+   (forall (R1 R2 : Type) (RR : R1 -> R2 -> Prop) (t1 : itree (D1 +' E1) R1) (t2 : itree (D2 +' E2) R2),
+       rutt_err (sum_prerel RPreInv RPre) (sum_postrel RPostInv RPost) RR t1 t2 ->
+       rutt_err RPre RPost RR (interp_mrec bodies1 t1) (interp_mrec bodies2 t2)).
+Proof.
+  move=> hrec R1 R2 RR t1 t2 ht.
+  apply interp_mrec_rutt with (RPreInv := RPreInv) (RPostInv := RPostInv).
+  + admit. (* this is hrec modulo extentional equality *)
+  admit. (* this is ht modulo extentional equality *)
+Admitted.
+
+Lemma rutt_err_weaken {E1 E2: Type -> Type}
+  {HasErr1: ErrEvent -< E1} {wE1 : with_Error E1}
+  {HasErr2: ErrEvent -< E2} {wE2 : with_Error E2}
+  {O1 O2 : Type}
+  (RpreInv : prerel E1 E2)
+  (RpostInv: postrel E1 E2)
+  (post post' : O1 -> O2 -> Prop) t1 t2 :
+  (forall o1 o2, post o1 o2 -> post' o1 o2) ->
+  rutt_err RpreInv RpostInv post t1 t2 ->
+  rutt_err RpreInv RpostInv post' t1 t2.
+Admitted.
+
+Definition rel (I1 I2 : Type) := I1 -> I2 -> Prop.
+
+Definition relIO (I1 I2 O1 O2 : Type) := I1 -> I2 -> O1 -> O2 -> Prop.
+
+Section REQUIV.
+
+Context {E:Set}.
+
+Definition fresult T1 T2 := T1 -> result E T2.
+
+Definition requiv_io {I1 I2 O1 O2}
+   (P : rel I1 I2) (F1 : fresult I1 O1) (F2 : fresult I2 O2) (Q : relIO I1 I2 O1 O2) :=
+  forall i1 i2 o1, P i1 i2 -> F1 i1 = ok o1 -> exists2 o2, F2 i2 = ok o2 & Q i1 i2 o1 o2.
+
+Definition requiv {I1 I2 O1 O2}
+   (P : rel I1 I2) (F1 : fresult I1 O1) (F2 : fresult I2 O2) (Q : rel O1 O2) :=
+  requiv_io P F1 F2 (fun _ _ => Q).
+
+Lemma requiv_io_weaken {I1 I2 O1 O2} (P P' : rel I1 I2) (Q Q': relIO I1 I2 O1 O2) F1 F2 :
+  (forall i1 i2, P' i1 i2 -> P i1 i2) ->
+  (forall i1 i2 o1 o2, P' i1 i2 -> Q i1 i2 o1 o2 -> Q' i1 i2 o1 o2) ->
+  requiv_io P F1 F2 Q ->
+  requiv_io P' F1 F2 Q'.
+Proof.
+  move=> hP'P hQQ' h i1 i2 o1 hP' hF1.
+  have [o2 -> hQ]:= h _ _ _ (hP'P _ _ hP') hF1; eauto.
+Qed.
+
+Lemma requiv_weaken {I1 I2 O1 O2} (P P' : rel I1 I2) (Q Q': rel O1 O2) F1 F2 :
+  (forall i1 i2, P' i1 i2 -> P i1 i2) ->
+  (forall o1 o2, Q o1 o2 -> Q' o1 o2) ->
+  requiv P F1 F2 Q ->
+  requiv P' F1 F2 Q'.
+Proof. move=> hP'P hQQ'; apply requiv_io_weaken => //; auto. Qed.
+
+Lemma requiv_io_ok {I1 I2} (P:rel I1 I2) (Q: relIO I1 I2 I1 I2):
+  (forall i1 i2, P i1 i2 -> Q i1 i2 i1 i2) ->
+  requiv_io P (@Ok _ _) (@Ok _ _) Q.
+Proof. by move=> hPQ i1 i2 o1 hQ [<-]; exists i2 => //; apply hPQ. Qed.
+
+Lemma requiv_ok {I1 I2} (Q:rel I1 I2) : requiv Q (@Ok _ _) (@Ok _ _) Q.
+Proof. by apply requiv_io_ok. Qed.
+
+Lemma requiv_io_err {I1 I2 O1 O2} (P:rel I1 I2) (Q: relIO I1 I2 O1 O2) (Err : E) F :
+  requiv_io P (fun i1 => Error Err) F Q.
+Proof. by move=> ?. Qed.
+
+Lemma requiv_err {I1 I2 O1 O2} (P:rel I1 I2) (Q: rel O1 O2) (Err : E) F :
+  requiv P (fun i1 => Error Err) F Q.
+Proof. apply requiv_io_err. Qed.
+
+Lemma requiv_io_bind {I1 I2 T1 T2 O1 O2}
+  (R : relIO I1 I2 T1 T2)
+  (P : rel I1 I2)
+  (Q : relIO I1 I2 O1 O2) F1 F1' F2 F2' :
+  requiv_io P F1 F2 R ->
+  (forall i1 i2, P i1 i2 -> requiv (R i1 i2) F1' F2' (Q i1 i2)) ->
+  requiv_io P (fun i => F1 i >>r= F1') (fun i => F2 i >>r= F2') Q.
+Proof.
+  move=> h h' i1 i2 o1 hP; t_xrbindP => t1 /(h _ _ _ hP) [t2 -> /= hR].
+  by apply: h'.
+Qed.
+
+Lemma requiv_bind {I1 I2 T1 T2 O1 O2}
+  (R : rel T1 T2)
+  (P : rel I1 I2)
+  (Q : rel O1 O2) F1 F1' F2 F2' :
+  requiv P F1 F2 R ->
+  requiv R F1' F2' Q ->
+  requiv P (fun i => F1 i >>r= F1') (fun i => F2 i >>r= F2') Q.
+Proof. by move=> h h'; apply requiv_io_bind with (R:= fun _ _ => R). Qed.
+
+Lemma requiv_bind2 {I1 I2 U1 U2 T1 T2 O1 O2}
+  (R : rel T1 T2) (P : rel I1 I2) (Q : rel O1 O2)
+  (F1 : U1 -> I1 -> result E T1) (F1' : T1 -> I1 -> result E O1)
+  (F2 : U2 -> I2 -> result E T2) (F2' : T2 -> I2 -> result E O2)
+  u1 u2 :
+  requiv P (F1 u1) (F2 u2) R ->
+  (forall t1 t2, R t1 t2 -> requiv P (F1' t1) (F2' t2) Q) ->
+  requiv P (fun i => Let t := F1 u1 i in F1' t i)
+           (fun i => Let t := F2 u2 i in F2' t i) Q.
+Proof.
+  move=> hF hF' i1 i2 o1 hP; t_xrbindP.
+  by move => t1 /(hF _ _ _ hP) [t2 -> /hF'] /=; apply.
+Qed.
+
+Lemma requiv_eq {I O} (F: fresult I O) : requiv eq F F eq.
+Proof. move=> i _ o <-; eauto. Qed.
+
+Lemma requiv_mapM {I1 I2 O1 O2} (P : rel I1 I2) (Q : rel O1 O2) F1 F2 :
+  requiv P F1 F2 Q ->
+  requiv (List.Forall2 P) (mapM F1) (mapM F2) (List.Forall2 Q).
+Proof.
+  move=> heqv s1; elim: s1 => [ | i1 is1 hrec] [ | i2 is2] os /List_Forall2_inv //=.
+  + by move=> _ [<-]; eauto.
+  move=> [hP halli]; t_xrbindP => o1 ho1 os1 hos1 <-.
+  have [o2 -> /= hQ] := heqv _ _ _ hP ho1.
+  have [os2 -> /= hallo] := hrec _ _ halli hos1; eauto.
+Qed.
+
+Lemma requiv_fold2 {A1 B1 A2 B2 R1 R2} (Err : E)
+  (I: rel R1 R2) (PA : rel A1 A2) (PB : rel B1 B2)
+  (F1 : A1 -> B1 -> R1 -> result E R1) (F2 : A2 -> B2 -> R2 -> result E R2)
+  (la1 : seq A1) (la2 : seq A2) (lb1 : seq B1) (lb2 : seq B2) :
+  Forall2 PA la1 la2 ->
+  Forall2 PB lb1 lb2 ->
+  (forall a1 a2 b1 b2, PA a1 a2 -> PB b1 b2 -> requiv I (F1 a1 b1) (F2 a2 b2) I) ->
+  requiv I (fold2 Err F1 la1 lb1) (fold2 Err F2 la2 lb2) I.
+Proof.
+  move=> halla hallb hF.
+  elim: halla lb1 lb2 hallb => {la1 la2}.
+  + by move=> _ _ [] => //=; apply requiv_ok.
+  move=> a1 a2 la1 la2 hPA halla hrec _ _ [] => //= b1 b2 lb1 lb2 hPB hallb.
+  apply requiv_bind with I; auto.
+Qed.
+
+Lemma requiv_mapM_all2 {S1 S2 I1 I2 O1 O2} (PS : rel S1 S2) (P : rel I1 I2) (Q : rel O1 O2) F1 F2 is1 is2:
+  Forall2 P is1 is2 ->
+  (forall s1 s2, PS s1 s2 -> requiv P (F1 s1) (F2 s2) Q) ->
+  requiv PS (fun s => mapM (F1 s) is1) (fun s => mapM (F2 s) is2) (Forall2 Q).
+Proof.
+  move=> his hPQ s1 s2 o1 hPS.
+  by apply (requiv_mapM (hPQ _ _ hPS)).
+Qed.
+
+End REQUIV.
+
+Lemma requiv_to_bool : requiv value_uincl to_bool to_bool eq.
+Proof.
+  move=> v1 v2 b1 hu hb1.
+  have [b2 /= -> /value_uinclE /= [->]] := val_uincl_of_val (ty:= sbool) hu hb1; eauto.
+Qed.
+
+Lemma requiv_to_int : requiv value_uincl to_int to_int eq.
+Proof.
+  move=> v1 v2 i1 hu hi1.
+  have [b2 /= -> /value_uinclE /= [->]] := val_uincl_of_val (ty:= sint) hu hi1; eauto.
+Qed.
+
+Lemma requiv_truncate_val ty :
+  requiv value_uincl (truncate_val ty) (truncate_val ty) value_uincl.
+Proof. move=> v1 v2 v1'; apply value_uincl_truncate. Qed.
+
+Class relEvent (E : Type -> Type) :=
+  { HasErr1  :: ErrEvent -< E
+  ; wE      :: with_Error E
+  ; RPreInv  :: prerel E E
+  ; RPostInv :: postrel E E }.
+
+Section IEQUIV.
+
+Context {E: Type -> Type} {rE : relEvent E}.
+
+Definition fitree E (I O : Type) := I -> itree E O.
+
+Definition iequiv_io {I1 I2 O1 O2}
+   (P : rel I1 I2) (F1 : fitree E I1 O1) (F2 : fitree E I2 O2) (Q : relIO I1 I2 O1 O2) :=
+  forall i1 i2, P i1 i2 -> rutt_err RPreInv RPostInv (Q i1 i2) (F1 i1) (F2 i2).
+
+Definition iequiv {I1 I2 O1 O2}
+   (P : rel I1 I2) (F1 : fitree E I1 O1) (F2 : fitree E I2 O2) (Q : rel O1 O2) :=
+   iequiv_io P F1 F2 (fun i1 i2 => Q).
+
+Lemma iequiv_io_weaken {I1 I2 O1 O2} (P P' : rel I1 I2) (Q Q': relIO I1 I2 O1 O2) F1 F2 :
+  (forall i1 i2, P' i1 i2 -> P i1 i2) ->
+  (forall i1 i2 o1 o2, P' i1 i2 -> Q i1 i2 o1 o2 -> Q' i1 i2 o1 o2) ->
+  iequiv_io P F1 F2 Q ->
+  iequiv_io P' F1 F2 Q'.
+Proof.
+  move=> hP'P hQQ' heqv i1 i2 hP'.
+  apply rutt_err_weaken with (Q i1 i2).
+  + by move=> >; apply hQQ'.
+  by apply/heqv/hP'P.
+Qed.
+
+Lemma iequiv_weaken {I1 I2 O1 O2} (P P' : rel I1 I2) (Q Q': rel O1 O2) F1 F2 :
+  (forall i1 i2, P' i1 i2 -> P i1 i2) ->
+  (forall o1 o2, Q o1 o2 -> Q' o1 o2) ->
+  iequiv P F1 F2 Q ->
+  iequiv P' F1 F2 Q'.
+Proof. move=> hP hQ; apply iequiv_io_weaken => // > _; apply hQ. Qed.
+
+Lemma iequiv_io_ret {I1 I2} (P: rel I1 I2) (Q : relIO I1 I2 I1 I2) :
+  (forall i1 i2, P i1 i2 -> Q i1 i2 i1 i2) ->
+  iequiv_io P (fun i => Ret i) (fun i => Ret i) Q.
+Proof. by move=> hPQ i1 i2 hP; apply/rutt_Ret/hPQ. Qed.
+
+Lemma iequiv_ret {I1 I2} (Q: rel I1 I2) :
+  iequiv Q (fun i => Ret i) (fun i => Ret i) Q.
+Proof. by apply iequiv_io_ret. Qed.
+
+Lemma iequiv_io_bind {I1 I2 T1 T2 O1 O2}
+  (R : relIO I1 I2 T1 T2)
+  (P : rel I1 I2)
+  (Q : relIO I1 I2 O1 O2) F1 F1' F2 F2' :
+  iequiv_io P F1 F2 R ->
+  (forall i1 i2, P i1 i2 -> iequiv (R i1 i2) F1' F2' (Q i1 i2)) ->
+  iequiv_io P (fun i => t <- F1 i;; F1' t) (fun i => t <- F2 i;; F2' t) Q.
+Proof.
+  move=> h h' i1 i2 hP.
+  apply rutt_bind with (R i1 i2); first by apply h.
+  by move=> t1 t2 hR; apply h'.
+Qed.
+
+Lemma iequiv_bind {I1 I2 T1 T2 O1 O2}
+  (R : rel T1 T2)
+  (P : rel I1 I2)
+  (Q : rel O1 O2) F1 F1' F2 F2' :
+  iequiv P F1 F2 R ->
+  iequiv R F1' F2' Q ->
+  iequiv P (fun i => t <- F1 i;; F1' t) (fun i => t <- F2 i;; F2' t) Q.
+Proof. by move=> h h'; apply iequiv_io_bind with (R := fun t1 t2 => R). Qed.
+
+End IEQUIV.
+
+(* Definition of a relational logic over program *)
+
+Section WSW.
+
+Context
+  {syscall_state : Type}
+  {ep : EstateParams syscall_state}
+  {spp : SemPexprParams}
+  {asm_op: Type}
+  {sip : SemInstrParams asm_op syscall_state}
+  {pT1 pT2 : progT}
+  {wsw1 wsw2: WithSubWord}
+  {scP1 : semCallParams (wsw:= wsw1) (pT := pT1)}
+  {scP2 : semCallParams (wsw:= wsw2) (pT := pT2)}
+  {dc1 dc2: DirectCall}.
+
+Notation prog1 := (prog (pT := pT1)).
+Notation prog2 := (prog (pT := pT2)).
+
+Notation extra_val_t1 := (@extra_val_t pT1).
+Notation extra_val_t2 := (@extra_val_t pT2).
+
+Notation estate1 := (estate (wsw:=wsw1) (ep:=ep)).
+Notation estate2 := (estate (wsw:=wsw2) (ep:=ep)).
+
+Notation isem_fun1 := (isem_fun (wsw:=wsw1) (dc:=dc1) (ep:=ep) (spp:=spp) (sip:=sip) (pT:=pT1) (scP:= scP1)).
+Notation isem_fun2 := (isem_fun (wsw:=wsw2) (dc:=dc2) (ep:=ep) (spp:=spp) (sip:=sip) (pT:=pT2) (scP:= scP2)).
+
+Section IRESULT.
+Context {E: Type -> Type} {rE: relEvent E}.
+
+Lemma rutt_iresult (T1 T2:Type) (s1 : estate1) (s2 : estate2) (x1 : exec T1) (x2 : exec T2) (R : T1 -> T2 -> Prop) :
+  (forall v1, x1 = ok v1 -> exists2 v2, x2 = ok v2 & R v1 v2) ->
+  rutt_err RPreInv RPostInv R (iresult s1 x1) (iresult s2 x2).
+Proof.
+  case: x1 => [ v1 | e1] hok.
+  + have [v2 -> /=] := hok _ erefl.
+    by apply: rutt_Ret.
+  apply rutt_CutL => //.
+  by rewrite /ErrorCutoff /= is_error_has.
+Qed.
+
+End IRESULT.
+
+Class sem_call_2 {E : Type -> Type} {rE: relEvent E} :=
+ { sem_call1 : prog1 -> extra_val_t1 -> funname -> fstate -> itree E fstate
+ ; sem_call2 : prog2 -> extra_val_t2 -> funname -> fstate -> itree E fstate }.
+
+#[global]
+Instance sc2_full {E : Type -> Type} {rE: relEvent E} : sem_call_2 | 100 :=
+  {| sem_call1 := isem_fun1
+   ; sem_call2 := isem_fun2 |}.
+
+Section TR_MutualRec.
+
+Context (RPreF : funname -> funname -> fstate -> fstate -> Prop).
+Context (RPostF : funname -> funname -> fstate -> fstate -> fstate -> fstate -> Prop).
+
+Context {E: Type -> Type} {rE:relEvent E}.
+Notation recCall := (callE (funname * fstate) fstate).
+
+Definition RPreD {T1 T2} (d1 : recCall T1)
+                         (d2 : recCall T2) : Prop :=
+  match d1, d2 with
+  | Call (fn1, fs1), Call (fn2, fs2) => RPreF fn1 fn2 fs1 fs2
+  end.
+
+Check @callE.
+
+Definition RPostD {T1 T2} (d1 : recCall T1) (t1: T1) (d2 : recCall T2) (t2: T2) : Prop :=
+  match d1 in callE _ _ T1_ return T1_ -> T2 -> Prop with
+  | Call (fn1, fs1) =>
+    match d2 in callE _ _ T2_ return fstate -> T2_ -> Prop with
+    | Call (fn2, fs2) => RPostF fn1 fn2 fs1 fs2
+    end
+  end t1 t2.
+
+Definition relEvent_recCall : relEvent (recCall +' E).
+econstructor.
++ apply with_Error_suml.
++ exact (sum_prerel (@RPreD) RPreInv).
++ exact (sum_postrel (@RPostD) RPostInv).
+Defined.
+
+Definition sc2_rec : sem_call_2 (rE := relEvent_recCall) :=
+  {| sem_call1 := rec_call (E:=E)
+   ; sem_call2 := rec_call (E:=E) |}.
+
+End TR_MutualRec.
+
+Section EQUIV_CORE.
+
+Context {E : Type -> Type} {rE: relEvent E}.
+
+Lemma iequiv_iresult (P Q : rel estate1 estate2) (F1 : estate1 -> exec estate1) (F2: estate2 -> exec estate2) :
+  requiv P F1 F2 Q ->
+  iequiv P (fun s => iresult s (F1 s)) (fun s => iresult s (F2 s)) Q.
+Proof. by move=> h s1 s2 hP; apply rutt_iresult => s1'; apply: h. Qed.
+
+Context {SC2 : sem_call_2} (p1 : prog1) (p2 : prog2) (ev1: extra_val_t1) (ev2 : extra_val_t2).
+
+Definition relPreF := funname -> funname -> fstate -> fstate -> Prop.
+Definition relPostF := funname -> funname -> fstate -> fstate -> fstate -> fstate -> Prop.
+
+Definition rel_e := rel pexpr pexpr.
+Definition rel_v := rel value value.
+Definition rel_vs := rel values values.
+Definition rel_c := rel estate1 estate2.
+
+Definition equiv_f (P : relPreF) (fn1 fn2 : funname) (Q:relPostF) :=
+  iequiv_io (P fn1 fn2) (sem_call1 p1 ev1 fn1) (sem_call2 p2 ev2 fn2) (Q fn1 fn2).
+
+Definition equiv_f_body (P : relPreF) (fn1 fn2 : funname) (Q:relPostF) :=
+  iequiv_io (P fn1 fn2)
+            (isem_funcall (dc:=dc1) sem_call1 p1 ev1 fn1) (isem_funcall (dc:=dc2) sem_call2 p2 ev2 fn2)
+            (Q fn1 fn2).
+
+Definition equiv (pre:rel_c) (c1 c2 : cmd) (post : rel_c) :=
+  iequiv pre (isem_cmd_ (dc:=dc1) sem_call1 p1 ev1 c1) (isem_cmd_ (dc:=dc2) sem_call2 p2 ev2 c2) post.
+
+Lemma equiv_weaken P1 P2 Q1 Q2 c1 c2 :
+  (forall s1 s2, P1 s1 s2 -> P2 s1 s2) ->
+  (forall s1 s2, Q2 s1 s2 -> Q1 s1 s2) ->
+  equiv P2 c1 c2 Q2 ->
+  equiv P1 c1 c2 Q1.
+Proof. by apply iequiv_weaken. Qed.
+
+Lemma equiv_cat (R P Q : rel_c) (c1 c1' c2 c2' : cmd) :
+  equiv P c1 c2 R ->
+  equiv R c1' c2' Q ->
+  equiv P (c1 ++ c1') (c2 ++ c2') Q.
+Proof.
+  move=> h h' s1 s2 hP; rewrite !isem_cmd_cat.
+  apply rutt_bind with R; first by apply h.
+  apply h'.
+Qed.
+
+Lemma equiv_nil Q : equiv Q [::] [::] Q.
+Proof. apply iequiv_ret. Qed.
+
+Lemma equiv_cons (R P Q : rel_c) (i1 i2 : instr) (c1 c2 : cmd) :
+  equiv P [::i1] [::i2] R ->
+  equiv R c1 c2 Q ->
+  equiv P (i1 :: c1) (i2 :: c2) Q.
+Proof. rewrite -(cat1s i1 c1) -(cat1s i2 c2); apply equiv_cat. Qed.
+
+Lemma equiv_assgn (Rv Rtr: rel_v) (P Q : rel_c) ii1 x1 tg1 ty1 e1 ii2 x2 tg2 ty2 e2 :
+  requiv P (fun s => sem_pexpr true (p_globs p1) s e1)
+           (fun s => sem_pexpr true (p_globs p2) s e2) Rv ->
+  requiv Rv (truncate_val ty1) (truncate_val ty2) Rtr ->
+  (forall v1 v2, Rtr v1 v2 ->
+    requiv P (write_lval true (p_globs p1) x1 v1) (write_lval true (p_globs p2) x2 v2) Q) ->
+  equiv P [:: MkI ii1 (Cassgn x1 tg1 ty1 e1)] [:: MkI ii2 (Cassgn x2 tg2 ty2 e2)] Q.
+Proof.
+  move=> he htr hwr; rewrite /equiv /isem_cmd_ /=.
+  apply iequiv_bind with Q; last apply iequiv_ret.
+  apply iequiv_iresult; rewrite /sem_assgn.
+  move=> s1 s2 s1' hP.
+  t_xrbindP => v1 /(he _ _ _ hP) [v2 -> /= hv] v1' /(htr _ _ _ hv) [v2' ->] hv' /=.
+  by apply hwr.
+Qed.
+
+Lemma equiv_assgn_eq (P Q : rel_c) ii1 x1 tg1 ty e1 ii2 x2 tg2 e2 :
+  requiv P (fun s => sem_pexpr true (p_globs p1) s e1)
+           (fun s => sem_pexpr true (p_globs p2) s e2) eq ->
+  (forall v, requiv P (write_lval true (p_globs p1) x1 v) (write_lval true (p_globs p2) x2 v) Q) ->
+  equiv P [:: MkI ii1 (Cassgn x1 tg1 ty e1)] [:: MkI ii2 (Cassgn x2 tg2 ty e2)] Q.
+Proof.
+  move=> he hx; apply equiv_assgn with eq eq => //.
+  + by apply requiv_eq.
+  by move=> > <-; apply hx.
+Qed.
+
+Lemma equiv_assgn_uincl (P Q : rel_c) ii1 x1 tg1 ty e1 ii2 x2 tg2 e2 :
+  requiv P (fun s => sem_pexpr true (p_globs p1) s e1)
+           (fun s => sem_pexpr true (p_globs p2) s e2) value_uincl ->
+  (forall v1 v2, value_uincl v1 v2 ->
+    requiv P (write_lval true (p_globs p1) x1 v1) (write_lval true (p_globs p2) x2 v2) Q) ->
+  equiv P [:: MkI ii1 (Cassgn x1 tg1 ty e1)] [:: MkI ii2 (Cassgn x2 tg2 ty e2)] Q.
+Proof. move=> he; apply equiv_assgn with value_uincl => //; apply requiv_truncate_val. Qed.
+
+Lemma equiv_opn (Rve Rvo : rel_vs) P Q ii1 xs1 at1 o1 es1 ii2 xs2 at2 o2 es2 :
+  requiv P (fun s => sem_pexprs true (p_globs p1) s es1)
+           (fun s => sem_pexprs true (p_globs p2) s es2) Rve ->
+  requiv Rve (exec_sopn o1) (exec_sopn o2) Rvo ->
+  (forall vs1 vs2,
+    Rvo vs1 vs2 -> requiv P (fun s1 => write_lvals true (p_globs p1) s1 xs1 vs1)
+                            (fun s2 => write_lvals true (p_globs p2) s2 xs2 vs2) Q) ->
+  equiv P [:: MkI ii1 (Copn xs1 at1 o1 es1)] [:: MkI ii2 (Copn xs2 at2 o2 es2)] Q.
+Proof.
+  move=> he ho hwr; rewrite /equiv /isem_cmd_ /=.
+  apply iequiv_bind with Q; last apply iequiv_ret.
+  apply iequiv_iresult.
+  move=> s1 s2 s1' hP; rewrite /sem_sopn.
+  t_xrbindP => vr1 v1 /(he _ _ _ hP) [v2 -> /= hv]  /(ho _ _ _ hv) [v2' ->] hv' /=.
+  by apply hwr.
+Qed.
+
+Lemma equiv_opn_eq P Q ii1 xs1 at1 o es1 ii2 xs2 at2 es2 :
+  requiv P (fun s => sem_pexprs true (p_globs p1) s es1)
+           (fun s => sem_pexprs true (p_globs p2) s es2) eq ->
+  (forall vs,
+    requiv P (fun s1 => write_lvals true (p_globs p1) s1 xs1 vs)
+             (fun s2 => write_lvals true (p_globs p2) s2 xs2 vs) Q) ->
+  equiv P [:: MkI ii1 (Copn xs1 at1 o es1)] [:: MkI ii2 (Copn xs2 at2 o es2)] Q.
+Proof.
+  move=> he hx; apply equiv_opn with eq eq => //.
+  + by apply requiv_eq.
+  by move=> > <-; apply hx.
+Qed.
+
+Lemma requiv_exec_sopn o :
+  requiv (Forall2 value_uincl) (exec_sopn o) (exec_sopn o) (Forall2 value_uincl).
+Proof. move=> vs1 vs2 vs1'; apply vuincl_exec_opn. Qed.
+
+Lemma equiv_opn_uincl P Q ii1 xs1 at1 o es1 ii2 xs2 at2 es2 :
+  requiv P (fun s => sem_pexprs true (p_globs p1) s es1)
+           (fun s => sem_pexprs true (p_globs p2) s es2) (Forall2 value_uincl) ->
+  (forall vs1 vs2,
+    Forall2 value_uincl vs1 vs2 ->
+    requiv P (fun s1 => write_lvals true (p_globs p1) s1 xs1 vs1)
+             (fun s2 => write_lvals true (p_globs p2) s2 xs2 vs2) Q) ->
+  equiv P [:: MkI ii1 (Copn xs1 at1 o es1)] [:: MkI ii2 (Copn xs2 at2 o es2)] Q.
+Proof.
+  move=> he; apply equiv_opn with (Forall2 value_uincl) => //; apply requiv_exec_sopn.
+Qed.
+
+Lemma equiv_syscall Rv Ro P Q ii1 xs1 sc1 es1 ii2 xs2 sc2 es2 :
+  requiv P (fun s => sem_pexprs true (p_globs p1) s es1)
+           (fun s => sem_pexprs true (p_globs p2) s es2) Rv ->
+  (forall vs1 vs2,
+     Rv vs1 vs2 ->
+     requiv P (fun (s:estate1) => fexec_syscall (scP:=scP1) sc1 (mk_fstate vs1 s))
+              (fun (s:estate2) => fexec_syscall sc2 (mk_fstate vs2 s)) Ro)->
+  (forall fs1 fs2,
+    Ro fs1 fs2 ->
+    requiv P (upd_estate true (p_globs p1) xs1 fs1)
+             (upd_estate true (p_globs p2) xs2 fs2) Q) ->
+  equiv P [:: MkI ii1 (Csyscall xs1 sc1 es1)] [:: MkI ii2 (Csyscall xs2 sc2 es2)] Q.
+Proof.
+  move=> he ho hwr; rewrite /equiv /isem_cmd_ /=.
+  apply iequiv_bind with Q; last apply iequiv_ret.
+  apply iequiv_iresult.
+  move=> s1 s2 s1' hP; rewrite /sem_syscall.
+  t_xrbindP => vs1 /(he _ _ _ hP) [vs2 -> /= hvs] fs1.
+  by move=> /(ho _ _ hvs _ _ _ hP) [fs2 -> /hwr /=]; apply.
+Qed.
+
+Lemma equiv_syscall_eq P Q ii1 xs1 sc1 es1 ii2 sc2 xs2 es2 :
+  (forall s1 s2, P s1 s2 -> escs s1 = escs s2 /\ emem s1 = emem s2) ->
+  requiv P (fun s => sem_pexprs true (p_globs p1) s es1)
+           (fun s => sem_pexprs true (p_globs p2) s es2) eq ->
+  requiv eq (fexec_syscall (scP:=scP1) sc1)
+            (fexec_syscall (scP:=scP2) sc2) eq ->
+  (forall fs,
+    requiv P (upd_estate true (p_globs p1) xs1 fs)
+             (upd_estate true (p_globs p2) xs2 fs) Q) ->
+  equiv P [:: MkI ii1 (Csyscall xs1 sc1 es1)] [:: MkI ii2 (Csyscall xs2 sc2 es2)] Q.
+Proof.
+  move=> heq he hsc hx.
+  apply equiv_syscall with eq eq => //.
+  + by rewrite /mk_fstate => > <- s1 s2 fs1 /heq [<- <-]; apply hsc.
+  move=> > <-; apply hx.
+Qed.
+
+Definition fs_uincl (fs1 fs2: fstate) :=
+  [/\ fs1.(fscs) = fs2.(fscs)
+    , fs1.(fmem) = fs2.(fmem)
+    & Forall2 value_uincl fs1.(fvals) fs2.(fvals)].
+
+Lemma equiv_syscall_uincl P Q ii1 xs1 sc1 es1 ii2 sc2 xs2 es2 :
+  (forall s1 s2, P s1 s2 -> escs s1 = escs s2 /\ emem s1 = emem s2) ->
+  requiv P (fun s => sem_pexprs true (p_globs p1) s es1)
+           (fun s => sem_pexprs true (p_globs p2) s es2) (Forall2 value_uincl) ->
+  requiv fs_uincl (fexec_syscall (scP:=scP1) sc1)
+                  (fexec_syscall (scP:=scP2) sc2) fs_uincl ->
+  (forall fs1 fs2,
+    fs_uincl fs1 fs2 ->
+    requiv P (upd_estate true (p_globs p1) xs1 fs1)
+             (upd_estate true (p_globs p2) xs2 fs2) Q) ->
+  equiv P [:: MkI ii1 (Csyscall xs1 sc1 es1)] [:: MkI ii2 (Csyscall xs2 sc2 es2)] Q.
+Proof.
+  move=> heq he hsc.
+  apply equiv_syscall with (Forall2 value_uincl) => //.
+  by rewrite /mk_fstate => vs1 vs2 hu s1 s2 fs1 /heq [<- <-]; apply hsc.
+Qed.
+
+Lemma equiv_if_full P Q ii1 e1 c1 c1' ii2 e2 c2 c2' :
+  requiv P (sem_cond (p_globs p1) e1) (sem_cond (p_globs p2) e2) eq ->
+  equiv (fun s1 s2 => [/\ P s1 s2, sem_cond (p_globs p1) e1 s1 = ok true & sem_cond (p_globs p2) e2 s2 = ok true])
+        c1 c2 Q ->
+  equiv (fun s1 s2 => [/\ P s1 s2, sem_cond (p_globs p1) e1 s1 = ok false & sem_cond (p_globs p2) e2 s2 = ok false])
+        c1' c2' Q ->
+  equiv P [:: MkI ii1 (Cif e1 c1 c1')] [:: MkI ii2 (Cif e2 c2 c2')] Q.
+Proof.
+  move=> he hc hc' s1 s2 hP; rewrite /isem_cmd_ /=.
+  apply rutt_bind with Q; last by move=> >; apply rutt_Ret.
+  apply rutt_bind with (fun b1 b2 =>
+     [/\ b1 = b2, sem_cond (p_globs p1) e1 s1 = ok b1 & sem_cond (p_globs p2) e2 s2 = ok b2]).
+  + by apply/rutt_iresult => b1 he1; have [b2 he2 heq] := he _ _ _ hP he1; exists b2.
+  by move=> [] _ [<- ??]; [apply hc | apply hc'].
+Qed.
+
+Lemma equiv_if P Q ii1 e1 c1 c1' ii2 e2 c2 c2' :
+  requiv P (sem_cond (p_globs p1) e1) (sem_cond (p_globs p2) e2) eq ->
+  equiv P c1 c2 Q ->
+  equiv P c1' c2' Q ->
+  equiv P [:: MkI ii1 (Cif e1 c1 c1')] [:: MkI ii2 (Cif e2 c2 c2')] Q.
+Proof.
+  move=> hcond hc hc'; apply equiv_if_full => //.
+  + by apply: equiv_weaken hc => // > [].
+  by apply: equiv_weaken hc' => // > [].
+Qed.
+
+Lemma sem_cond_uincl P e1 e2 :
+  requiv P (fun (s:estate1) => sem_pexpr true (p_globs p1) s e1)
+           (fun (s:estate2) => sem_pexpr true (p_globs p2) s e2) value_uincl ->
+  requiv P (sem_cond (p_globs p1) e1) (sem_cond (p_globs p2) e2) eq.
+Proof.
+  move=> he; rewrite /sem_cond.
+  apply: requiv_bind requiv_to_bool; apply he.
+Qed.
+
+Lemma equiv_if_uincl P Q ii1 e1 c1 c1' ii2 e2 c2 c2' :
+  requiv P (fun (s:estate1) => sem_pexpr true (p_globs p1) s e1)
+           (fun (s:estate2) => sem_pexpr true (p_globs p2) s e2) value_uincl ->
+  equiv P c1 c2 Q ->
+  equiv P c1' c2' Q ->
+  equiv P [:: MkI ii1 (Cif e1 c1 c1')] [:: MkI ii2 (Cif e2 c2 c2')] Q.
+Proof. move=> /sem_cond_uincl; apply equiv_if. Qed.
+
+Lemma equiv_if_eq P Q ii1 e1 c1 c1' ii2 e2 c2 c2' :
+  requiv P (fun (s:estate1) => sem_pexpr true (p_globs p1) s e1)
+           (fun (s:estate2) => sem_pexpr true (p_globs p2) s e2) eq ->
+  equiv P c1 c2 Q ->
+  equiv P c1' c2' Q ->
+  equiv P [:: MkI ii1 (Cif e1 c1 c1')] [:: MkI ii2 (Cif e2 c2 c2')] Q.
+Proof. by move=> he; apply equiv_if_uincl; apply: requiv_weaken he => // > <-. Qed.
+
+Lemma equiv_for P Pi ii1 i1 d lo1 hi1 c1 ii2 i2 lo2 hi2 c2 :
+  requiv P (sem_bound (p_globs p1) lo1 hi1) (sem_bound (p_globs p2) lo2 hi2) eq ->
+  (forall i : Z, requiv P (write_var true i1 (Vint i)) (write_var true i2 (Vint i)) Pi) ->
+  equiv Pi c1 c2 P ->
+  equiv P [:: MkI ii1 (Cfor i1 (d, lo1, hi1) c1)] [:: MkI ii2 (Cfor i2 (d, lo2, hi2) c2)] P.
+Proof.
+  move=> hbound hwi hc s1 s2 hP; rewrite /isem_cmd_ /=.
+  apply rutt_bind with P; last by move=> >; apply rutt_Ret.
+  apply rutt_bind with eq.
+  + by apply rutt_iresult => >; apply hbound.
+  move=> [vlo vhi] _ <- /=; elim: wrange s1 s2 hP=> [|j js hrec] /= s1 s2 hP.
+  + by apply rutt_Ret.
+  apply rutt_bind with Pi.
+  + by apply rutt_iresult => >; apply hwi.
+  move=> r1 r2 hPi; apply rutt_bind with P => //.
+  by apply hc.
+Qed.
+
+Lemma requiv_sem_bound (P : rel_c) lo1 hi1 lo2 hi2 :
+  requiv P (fun (s:estate1) => sem_pexpr true (p_globs p1) s lo1)
+           (fun (s:estate2) => sem_pexpr true (p_globs p2) s lo2) value_uincl ->
+  requiv P (fun (s:estate1) => sem_pexpr true (p_globs p1) s hi1)
+           (fun (s:estate2) => sem_pexpr true (p_globs p2) s hi2) value_uincl ->
+  requiv P (sem_bound (p_globs p1) lo1 hi1) (sem_bound (p_globs p2) lo2 hi2) eq.
+Proof.
+  move=> hlo hhi; rewrite /sem_bound.
+  have h : forall e1 e2,
+    requiv P (fun (s:estate1) => sem_pexpr true (p_globs p1) s e1)
+             (fun (s:estate2) => sem_pexpr true (p_globs p2) s e2) value_uincl ->
+    requiv P (fun (s:estate1) => sem_pexpr true (p_globs p1) s e1 >>r= to_int)
+             (fun (s:estate2) => sem_pexpr true (p_globs p2) s e2 >>r= to_int) eq.
+  + by move=> e1 e2 he; apply: requiv_bind requiv_to_int; apply he.
+  move=> s1 s2 lh1 hP.
+  apply rbindP => vlo /(h _ _ hlo _ _ _ hP) [_ -> <-].
+  apply rbindP => vhi /(h _ _ hhi _ _ _ hP) [_ -> <-] [<-] /=; eauto.
+Qed.
+
+Lemma equiv_for_uincl P Pi ii1 i1 d lo1 hi1 c1 ii2 i2 lo2 hi2 c2 :
+  requiv P (fun (s:estate1) => sem_pexpr true (p_globs p1) s lo1)
+           (fun (s:estate2) => sem_pexpr true (p_globs p2) s lo2) value_uincl ->
+  requiv P (fun (s:estate1) => sem_pexpr true (p_globs p1) s hi1)
+           (fun (s:estate2) => sem_pexpr true (p_globs p2) s hi2) value_uincl ->
+  (forall i : Z, requiv P (write_var true i1 (Vint i)) (write_var true i2 (Vint i)) Pi) ->
+  equiv Pi c1 c2 P ->
+  equiv P [:: MkI ii1 (Cfor i1 (d, lo1, hi1) c1)] [:: MkI ii2 (Cfor i2 (d, lo2, hi2) c2)] P.
+Proof. by move=> hlo hhi; apply/equiv_for/requiv_sem_bound. Qed.
+
+Lemma equiv_for_eq P Pi ii1 i1 d lo1 hi1 c1 ii2 i2 lo2 hi2 c2 :
+  requiv P (fun (s:estate1) => sem_pexpr true (p_globs p1) s lo1)
+           (fun (s:estate2) => sem_pexpr true (p_globs p2) s lo2) eq ->
+  requiv P (fun (s:estate1) => sem_pexpr true (p_globs p1) s hi1)
+           (fun (s:estate2) => sem_pexpr true (p_globs p2) s hi2) eq ->
+  (forall i : Z, requiv P (write_var true i1 (Vint i)) (write_var true i2 (Vint i)) Pi) ->
+  equiv Pi c1 c2 P ->
+  equiv P [:: MkI ii1 (Cfor i1 (d, lo1, hi1) c1)] [:: MkI ii2 (Cfor i2 (d, lo2, hi2) c2)] P.
+Proof.
+  move=> hlo hhi; apply equiv_for_uincl.
+  + by apply: requiv_weaken hlo => // > <-.
+  by apply: requiv_weaken hhi => // > <-.
+Qed.
+
+Lemma equiv_while_full I I' ii1 al1 e1 c1 c1' ii2 al2 e2 c2 c2' :
+  equiv I c1 c2 I' ->
+  requiv I' (sem_cond (p_globs p1) e1) (sem_cond (p_globs p2) e2) eq ->
+  equiv (fun s1 s2 =>
+    [/\ I' s1 s2, sem_cond (p_globs p1) e1 s1 = ok true & sem_cond (p_globs p2) e2 s2 = ok true]) c1' c2' I ->
+  equiv I [:: MkI ii1 (Cwhile al1 c1 e1 c1')] [:: MkI ii2 (Cwhile al2 c2 e2 c2')]
+     (fun s1 s2 => [/\ I' s1 s2, sem_cond (p_globs p1) e1 s1 = ok false & sem_cond (p_globs p2) e2 s2 = ok false]).
+Proof.
+  move=> hc hcond hc' s1 s2 hI; rewrite /isem_cmd_ /=.
+  set Q := (fun s1 s2 =>
+    [/\ I' s1 s2, sem_cond (p_globs p1) e1 s1 = ok false & sem_cond (p_globs p2) e2 s2 = ok false]).
+  apply rutt_bind with Q; last by move=> >; apply rutt_Ret.
+  rewrite /isem_while; apply XRuttFacts.rutt_iter with (RI := I) => //.
+  move=> {}s1 {}s2 {}hI; rewrite /isem_while_loop.
+  apply rutt_bind with I'; first by apply hc.
+  move=> {hI} {}s1 {}s2 hI'.
+  apply rutt_bind with
+    (fun b1 b2 => [/\ b1 = b2, sem_cond (p_globs p1) e1 s1 = ok b1 & sem_cond (p_globs p2) e2 s2 = ok b2]).
+  + by apply/rutt_iresult => b1 he1; have [b2 he2 heq] := hcond _ _ _ hI' he1; exists b2.
+  move=> [] _ [<- he1 he2].
+  + apply rutt_bind with I; first by apply hc'.
+    by move=> r1 r2 hI; apply rutt_Ret; constructor.
+  by apply rutt_Ret; constructor.
+Qed.
+
+Lemma equiv_while I I' ii1 al1 e1 c1 c1' ii2 al2 e2 c2 c2' :
+  requiv I' (sem_cond (p_globs p1) e1) (sem_cond (p_globs p2) e2) eq ->
+  equiv I c1 c2 I' ->
+  equiv I' c1' c2' I ->
+  equiv I [:: MkI ii1 (Cwhile al1 c1 e1 c1')] [:: MkI ii2 (Cwhile al2 c2 e2 c2')] I'.
+Proof.
+  move=> hcond hc hc'.
+  apply equiv_weaken with (P2 := I)
+    (Q2 := fun s1 s2 =>
+      [/\ I' s1 s2, sem_cond (p_globs p1) e1 s1 = ok false & sem_cond (p_globs p2) e2 s2 = ok false]) => //.
+  + by move=> > [].
+  apply equiv_while_full => //.
+  by apply: equiv_weaken hc' => // > [].
+Qed.
+
+Lemma equiv_while_uincl I I' ii1 al1 e1 c1 c1' ii2 al2 e2 c2 c2' :
+  requiv I' (fun (s:estate1) => sem_pexpr true (p_globs p1) s e1)
+            (fun (s:estate2) => sem_pexpr true (p_globs p2) s e2) value_uincl ->
+  equiv I c1 c2 I' ->
+  equiv I' c1' c2' I ->
+  equiv I [:: MkI ii1 (Cwhile al1 c1 e1 c1')] [:: MkI ii2 (Cwhile al2 c2 e2 c2')] I'.
+Proof. move=> /sem_cond_uincl; apply equiv_while. Qed.
+
+Lemma equiv_while_eq I I' ii1 al1 e1 c1 c1' ii2 al2 e2 c2 c2' :
+  requiv I' (fun (s:estate1) => sem_pexpr true (p_globs p1) s e1)
+            (fun (s:estate2) => sem_pexpr true (p_globs p2) s e2) eq ->
+  equiv I c1 c2 I' ->
+  equiv I' c1' c2' I ->
+  equiv I [:: MkI ii1 (Cwhile al1 c1 e1 c1')] [:: MkI ii2 (Cwhile al2 c2 e2 c2')] I'.
+Proof. by move=> he; apply equiv_while_uincl; apply: requiv_weaken he => // > <-. Qed.
+
+Lemma equiv_call (Pf : relPreF) (Qf : relPostF) Rv P Q ii1 xs1 fn1 es1 ii2 xs2 fn2 es2 :
+  requiv P (fun s => sem_pexprs (~~ (@direct_call dc1)) (p_globs p1) s es1)
+           (fun s => sem_pexprs (~~ (@direct_call dc2)) (p_globs p2) s es2) Rv ->
+  (forall s1 s2 vs1 vs2,
+     P s1 s2 -> Rv vs1 vs2 ->
+     Pf fn1 fn2 (mk_fstate vs1 s1) (mk_fstate vs2 s2)) ->
+  equiv_f Pf fn1 fn2 Qf ->
+  (forall fs1 fs2 fr1 fr2,
+    Pf fn1 fn2 fs1 fs2 -> Qf fn1 fn2 fs1 fs2 fr1 fr2 ->
+    requiv P (upd_estate (~~ (@direct_call dc1)) (p_globs p1) xs1 fr1)
+             (upd_estate (~~ (@direct_call dc2)) (p_globs p2) xs2 fr2) Q) ->
+  equiv P [:: MkI ii1 (Ccall xs1 fn1 es1)] [:: MkI ii2 (Ccall xs2 fn2 es2)] Q.
+Proof.
+  move=> hes hPPf hCall hPQf s1 s2 hP; rewrite /isem_cmd_ /=.
+  apply rutt_bind with Q; last by move=> >; apply rutt_Ret.
+  apply rutt_bind with Rv.
+  + by apply rutt_iresult => >; apply: hes.
+  move=> vs1 vs2 hvs.
+  set fs1 := mk_fstate vs1 s1; set fs2 := mk_fstate vs2 s2.
+  apply rutt_bind with (Qf fn1 fn2 fs1 fs2).
+  + by apply/hCall/hPPf.
+  move=> fr1 fr2 hr; apply rutt_iresult => >.
+  apply (hPQf fs1 fs2 fr1 fr2) => //.
+  by apply hPPf.
+Qed.
+
+Definition isem_fun_body_hyp (RPreF:relPreF) fn1 fn2 (RPostF:relPostF) :=
+  forall fs1 fs2,
+  RPreF fn1 fn2 fs1 fs2 ->
+  forall fd1, get_fundef (p_funcs p1) fn1 = Some fd1 ->
+  exists2 fd2, get_fundef (p_funcs p2) fn2 = Some fd2 &
+    exists (P Q : rel_c),
+      forall s11, initialize_funcall (dc:=dc1) p1 ev1 fd1 fs1 = ok s11 ->
+      exists s21,
+        [/\ initialize_funcall (dc:=dc2) p2 ev2 fd2 fs2 = ok s21
+          , P s11 s21
+          , equiv P fd1.(f_body) fd2.(f_body) Q
+          & requiv Q (finalize_funcall (dc:=dc1) fd1) (finalize_funcall (dc:=dc2) fd2) (RPostF fn1 fn2 fs1 fs2)].
+
+Lemma equiv_fun_body RPreF fn1 fn2 RPostF :
+  isem_fun_body_hyp RPreF fn1 fn2 RPostF ->
+  equiv_f_body RPreF fn1 fn2 RPostF.
+Proof.
+  move=> hf fs1 fs2 hpre.
+  rewrite /isem_funcall.
+  have {}hf := hf _ _ hpre.
+  rewrite /iget_fundef.
+  apply rutt_bind with (fun fd1 fd2 => get_fundef (p_funcs p1) fn1 = Some fd1 /\
+                                        get_fundef (p_funcs p2) fn2 = Some fd2).
+  + case heq: get_fundef => [fd1 | ] /=.
+    + by have [fd2 -> _] := hf _ heq; apply rutt_Ret.
+    by apply rutt_CutL; rewrite /ErrorCutoff /= is_error_has.
+  move=> fd1 fd2 [hfd1 hfd2]; have := hf fd1 hfd1.
+  rewrite hfd2 => -[ _ [<- [P] [Q] {}hf]].
+  apply rutt_bind with (fun s1 s2 => initialize_funcall (dc:=dc1) p1 ev1 fd1 fs1 = ok s1 /\
+                                     initialize_funcall (dc:=dc2) p2 ev2 fd2 fs2 = ok s2).
+  + apply rutt_iresult.
+    by move=> s hs; have [s' [?]] := hf _ hs; eauto.
+  move=> s1 s1' [hs1 hs1']; have := hf _ hs1.
+  rewrite hs1' => -[?] [[<-] hP heqv hpost].
+  apply rutt_bind with Q.
+  + by apply heqv.
+  move=> r1 r2 hQ; apply rutt_iresult.
+  by move=> fr1; apply hpost.
+Qed.
+
+End EQUIV_CORE.
+
+Section EQUIV_FUN.
+
+Context {E : Type -> Type} {rE : relEvent E}.
+
+Context (p1 : prog1) (p2 : prog2) (ev1: extra_val_t1) (ev2 : extra_val_t2).
+
+Definition equiv_f_rec RPreF fn1 fn2 RPostF :=
+  equiv_f (rE:=relEvent_recCall RPreF RPostF) (SC2:=sc2_rec RPreF RPostF) p1 p2 ev1 ev2 RPreF fn1 fn2 RPostF.
+
+Definition equiv_rec (RPreF : relPreF) (RPostF : relPostF) P c1 c2 Q :=
+  equiv (rE:=relEvent_recCall RPreF RPostF) (SC2:=sc2_rec RPreF RPostF) p1 p2 ev1 ev2 P c1 c2 Q.
+
+Definition isem_fun_body_hyp_rec (RPreF:relPreF) fn1 fn2 (RPostF:relPostF) :=
+  forall fs1 fs2,
+  RPreF fn1 fn2 fs1 fs2 ->
+  forall fd1, get_fundef (p_funcs p1) fn1 = Some fd1 ->
+  exists2 fd2, get_fundef (p_funcs p2) fn2 = Some fd2 &
+    exists (P Q : rel_c),
+      forall s11, initialize_funcall (dc:=dc1) p1 ev1 fd1 fs1 = ok s11 ->
+      exists s21,
+        [/\ initialize_funcall (dc:=dc2) p2 ev2 fd2 fs2 = ok s21
+          , P s11 s21
+          , equiv_rec RPreF RPostF P fd1.(f_body) fd2.(f_body) Q
+          & requiv Q (finalize_funcall (dc:=dc1) fd1) (finalize_funcall (dc:=dc2) fd2) (RPostF fn1 fn2 fs1 fs2)].
+
+Lemma isem_fun_ind (RPreF : relPreF) (RPostF : relPostF) :
+  ((forall fn1 fn2, equiv_f_rec RPreF fn1 fn2 RPostF) ->
+   (forall fn1 fn2, isem_fun_body_hyp_rec RPreF fn1 fn2 RPostF)) ->
+  forall fn1 fn2,
+  equiv_f (rE:=rE) (SC2:=sc2_full) p1 p2 ev1 ev2 RPreF fn1 fn2 RPostF.
+Proof.
+  have hrec : (forall fn1 fn2, equiv_f_rec RPreF fn1 fn2 RPostF).
+  + move=> fn1' fn2' fs1' fs2' hpre'; apply rutt_trigger => //.
+    + by apply sum_prerel_inl.
+    by rewrite /RPostInv /= => fr1 fr2 h; dependent destruction h.
+    move=> /(_ hrec) hbody fn1 fn2 fs1 fs2 hpre.
+
+    unfold sem_call1, sem_call2. simpl. unfold isem_fun1, isem_fun2. simpl.
+
+    About interp_mrec_rutt.
+
+    unfold rec.
+    unfold mrec.
+    
+    apply interp_mrec_rutt_err with (RPreInv := @RPreD RPreF) (RPostInv := @RPostD RPostF).
+
+    intros.
+    unfold calling'. simpl.
+    destruct d1. destruct d2.
+    destruct p, p0.
+    unfold RPreD in H.
+    
+    unfold handle_recCall.
+    unfold isem_fun_rec.
+    unfold isem_funcall.
+    eapply rutt_trigger.
+    
+  + move=> {hpre fn1 fn2 fs1 fs2}.
+    move=> _ _ [fn1 fs1] [fn2 fs2] /= hpre.
+    by apply (equiv_fun_body (hbody fn1 fn2) hpre).
+  by apply (equiv_fun_body (hbody fn1 fn2) hpre).
+Qed.
+
+End EQUIV_FUN.
+
+End WSW.
+
+Section TEST.
+
+Context
+  {syscall_state : Type}
+  {ep : EstateParams syscall_state}
+  {spp : SemPexprParams}
+  {asm_op: Type}
+  {sip : SemInstrParams asm_op syscall_state}
+  {pT : progT}
+  {wsw: WithSubWord}
+  {scP : semCallParams}
+  {dc: DirectCall}.
+
+Context {E : Type -> Type} {rE : relEvent E}.
+
+Context (tr_lval : lval -> lval)
+        (tr_expr : pexpr -> pexpr).
+
+Local Notation tr_lvals ls := (map tr_lval ls).
+Local Notation tr_exprs es := (map tr_expr es).
+
+Fixpoint tr_i (i : instr) : instr :=
+  let: (MkI ii i) := i in
+  let i' :=
+    match i with
+    | Cassgn x tg ty e => Cassgn (tr_lval x) tg ty (tr_expr e)
+    | Copn xs tg o es =>
+        Copn (tr_lvals xs) tg o (tr_exprs es)
+    | Csyscall xs sc es =>
+        Csyscall (tr_lvals xs) sc (tr_exprs es)
+    | Cif e c1 c2 => Cif (tr_expr e) (map tr_i c1) (map tr_i c2)
+    | Cfor i (d, lo, hi) c => Cfor i (d, tr_expr lo, tr_expr hi) (map tr_i c)
+    | Cwhile a c1 e c2 => Cwhile a (map tr_i c1) (tr_expr e) (map tr_i c2)
+    | Ccall xs fn es => Ccall (tr_lvals xs) fn (tr_exprs es)
+    end in
+  MkI ii i'.
+
+Local Notation tr_c := (map tr_i).
+
+Definition tr_fundef (f: fundef) : fundef :=
+  {| f_info := f_info f
+   ; f_tyin := f_tyin f
+   ; f_params := f_params f
+   ; f_body := tr_c (f_body f)
+   ; f_tyout := f_tyout f
+   ; f_res := f_res f
+   ; f_extra := f_extra f |}.
+
+Context (p1 : prog) (ev:extra_val_t).
+
+Let p2 := map_prog tr_fundef p1.
+
+Definition RPreFeq (fn1 fn2 : funname) (fs1 fs2 : fstate) := fn1 = fn2 /\ fs1 = fs2.
+Definition RPostFeq (fn1 fn2 : funname) (fs1 fs2 fr1 fr2: fstate) := fr1 = fr2.
+
+Context (tr_exprP : forall wdb gd e,
+  requiv eq (fun s => sem_pexpr wdb gd s e) (fun s => sem_pexpr wdb gd s (tr_expr e)) eq).
+
+Context (tr_lvalP : forall wdb gd x v,
+   requiv eq (write_lval wdb gd x v) (write_lval wdb gd (tr_lval x) v) eq).
+
+Context (tr_exprsP : forall wdb gd es,
+   requiv eq ((sem_pexprs wdb gd)^~ es) ((sem_pexprs wdb gd)^~ (tr_exprs es)) eq).
+
+Context (tr_lvalsP : forall wdb gd x v,
+   requiv eq (fun s => write_lvals wdb gd s x v) (fun s => write_lvals wdb gd s (tr_lvals x) v) eq).
+
+Lemma eq_globs : p_globs p1 = p_globs p2.
+Proof. done. Qed.
+
+Lemma tr_updP wdb xs fs :
+  requiv eq (upd_estate wdb (p_globs p1) xs fs) (upd_estate wdb (p_globs p2) (tr_lvals xs) fs) eq.
+Admitted.
+
+Lemma Tr_fundefP fn : equiv_f p1 p2 ev ev RPreFeq fn fn RPostFeq.
+Proof.
+ apply isem_fun_ind => hrec {fn}.
+ move=> fn _ fs _ [<- <-] fd hget.
+ exists (tr_fundef fd).
+ + by rewrite get_map_prog hget.
+ move=> {hget}; exists eq, eq => s1 hinit.
+ exists s1; split => //; last first.
+ + by move=> s1' _ fr1 <- hfinal; exists fr1.
+ set Pi := fun (i:instr) => equiv_rec p1 p2 ev ev RPreFeq RPostFeq eq [::i] [::tr_i i] eq.
+ set Pr := fun (i:instr_r) => forall ii, Pi (MkI ii i).
+ set Pc := fun (c:cmd) => equiv_rec p1 p2 ev ev RPreFeq RPostFeq eq c (tr_c c) eq.
+ move=> {fn fs hinit}.
+ apply (cmd_rect (Pr := Pr) (Pi:=Pi) (Pc:=Pc)) => // {fd}.
+ + by apply equiv_nil.
+ + by move=> i c; apply equiv_cons.
+ + by move=> x tg ty e ii; apply equiv_assgn_eq.
+ + by move=> xs t o es ii; apply equiv_opn_eq.
+ + move=> xs o es ii; apply equiv_syscall_eq => //.
+   + by move=> > <-.
+   + by apply requiv_eq.
+   by apply tr_updP.
+ + by move=> e c1 c2 hc1 hc2 ii; apply equiv_if_eq.
+ + move=> j d lo hi c hc ii; apply equiv_for_eq with eq => //.
+   by move=> i s _ s' <-; eauto.
+ + by move=> al c e c' hc hc' ii; apply equiv_while_eq.
+ move=> xs f es ii; apply equiv_call with RPreFeq RPostFeq eq => //.
+ + by move=> > <- <-.
+ + by apply hrec.
+ move=> fs1 fs2 fr _ _ <-.
+ by apply tr_updP.
+Qed.
+
+End TEST.
+
